PDDL grounder implementation

Grounded_PDDL.thy
@@ -1,34 +1,119 @@
 theory Grounded_PDDL
 imports "AI_Planning_Languages_Semantics.PDDL_STRIPS_Semantics"
-    PDDL_Sema_Supplement
-    Utils
+    PDDL_Sema_Supplement Normalization_Definitions
+    Utils String_Shenanigans
 begin
 
-context wf_ast_domain begin
+type_synonym facty = "object atom formula"
 
-(* restrict types?
-  restrict objects, since they could only be used in init and goal?*)
+(* TODO split into wf_dom_grounder, dom_grounder, prob_grounder? *)
 
-fun grounded_ac :: "ast_action_schema \<Rightarrow> bool" where
-  "grounded_ac (Action_Schema n params pre effs) \<longleftrightarrow>
-    params = []"
+(* parameters for grounding: lists of achievable facts and applicable plan actions *)
 
-definition "grounded_dom \<equiv>
-  list_all1 grounded_ac (actions D)"
+(*fun fact_to_atom :: "fact \<Rightarrow> object atom formula" where
+  "fact_to_atom (p, args) = Atom (predAtm p args)"
+
+fun atom_to_fact :: "object atom formula \<Rightarrow> fact" where
+  "atom_to_fact (Atom (predAtm p args)) = (p, args)" |
+  "atom_to_fact \<phi> = undefined"*)
+
+fun arg_str :: "object list \<Rightarrow> string" where
+  "arg_str [] = ''''" |
+  "arg_str [Obj n] = n" |
+  "arg_str (Obj n # objs) = n @ ((CHR ''-'') # arg_str objs)"
+
+fun fact_str :: "object atom \<Rightarrow> string" where
+  "fact_str (predAtm (Pred n) args) = n @ ((CHR ''-'' # arg_str args))" |
+  "fact_str _ = undefined"
+
+fun ac_str :: "plan_action \<Rightarrow> string" where
+  "ac_str (PAction n args) = n @ (CHR ''-'' # arg_str args)"
+
+locale grounder = ast_problem +
+  fixes facts :: "facty list" and ops :: "plan_action list"
+begin
+
+definition "fact_ids \<equiv> nat_range (length facts)"
+definition "fact_prefix_pad \<equiv> length (show (length facts))" (* length facts - 1 is enough *)
+definition "op_ids \<equiv> nat_range (length ops)"
+definition "op_prefix_pad \<equiv> length (show (length ops))" (* length ops - 1 is enough *)
+
+fun grounded_pred :: "facty \<Rightarrow> nat \<Rightarrow> predicate" where
+  "grounded_pred (Atom a) i = Pred (padl fact_prefix_pad (show i) @ (CHR ''/'' # fact_str a))" |
+  "grounded_pred _ _ = undefined"
+
+abbreviation "gr_pred_ids \<equiv> map2 grounded_pred facts fact_ids"
+definition "fact_map \<equiv> map_of (zip (map un_Atom facts) gr_pred_ids)"
+
+fun map_fact :: "object atom \<Rightarrow> 'a atom" where
+  "map_fact a = predAtm (the (fact_map a)) []"
+
+(* fun grounded_pred_decl :: "facty \<Rightarrow> nat \<Rightarrow> predicate_decl" where
+  "grounded_pred_decl f i = PredDecl (grounded_pred f i) []" *)
+
+fun ga_pre :: "ground_action \<Rightarrow> term atom formula" where
+  "ga_pre (Ground_Action pre eff) = map_formula map_fact pre"
+
+fun ga_eff :: "ground_action \<Rightarrow> term ast_effect" where
+  "ga_eff (Ground_Action pre (Effect a d)) =
+    Effect (map (map_formula map_fact) a) (map (map_formula map_fact) d)"
+
+fun ground_ac_name :: "plan_action \<Rightarrow> nat \<Rightarrow> string" where
+  "ground_ac_name (PAction n args) i =
+    pad op_prefix_pad (show i) @ (CHR ''/'' # n) @ ((CHR ''-'' # arg_str args))"
+
+fun grounded_ac :: "plan_action \<Rightarrow> nat \<Rightarrow> ast_action_schema" where
+  "grounded_ac \<pi> i =
+    (let ga = resolve_instantiate \<pi> in
+    Action_Schema (ground_ac_name \<pi> i) [] (ga_pre ga) (ga_eff ga))"
+
+definition ground_dom :: "ast_domain" where
+  "ground_dom \<equiv> Domain
+    []
+    (map (\<lambda>p. PredDecl p []) gr_pred_ids)
+    []
+    (map2 grounded_ac ops op_ids)"
+
+definition ground_prob :: "ast_problem" where
+  "ground_prob \<equiv> Problem
+    ground_dom
+    []
+    (map (map_formula map_fact) (init P))
+    (map_formula map_fact (goal P))"
+
+
 end
+
+locale wf_grounder = grounder +
+  assumes
+    wf_problem and
+    facts_dist: "distinct facts" and
+    all_facts: "set facts \<supseteq> {a. achievable a}" and
+    ops_dist: "distinct ops" and
+    ops_correct: "set ops \<supseteq> {\<pi>. applicable \<pi>}"
+begin end
+
+sublocale wf_grounder \<subseteq> wf_ast_problem P
+  apply (unfold_locales)
+  using wf_grounder_axioms wf_grounder_def by blast
+
+
+subsection \<open> locale setup \<close>
 
 locale grounded_domain = wf_ast_domain +
   assumes grounded_dom: grounded_dom
 
 locale grounded_problem = wf_ast_problem +
-  assumes grounded_dom: grounded_dom
+  assumes grounded_prob: grounded_prob
 
 sublocale grounded_problem \<subseteq> grounded_domain D
-  using grounded_dom by (unfold_locales) simp
+  using grounded_prob grounded_prob_def by (unfold_locales) simp
 
+
+subsection \<open> Properties of grounded tasks \<close>
 
 lemma (in grounded_problem)
-  assumes "wf_plan_action (PlanAction n args)"
+  assumes "wf_plan_action (PAction n args)"
   shows "args = []"
   oops
 
@@ -36,7 +121,7 @@ lemma (in grounded_problem)
   assumes "wf_plan_action \<pi>"
   obtains ac where
     "ac \<in> set (actions D)"
-    "wf_plan_action (PlanAction ac [])"
+    "wf_plan_action (PAction n [])"
     "resolve_instantiate \<pi> = instantiate_action_schema ac []"
   oops
 
@@ -44,6 +129,23 @@ lemma (in grounded_problem)
 
 
 
+subsection \<open> Code Setup \<close>
+
+lemmas pddl_ground_code =
+  grounder.fact_ids_def
+  grounder.fact_prefix_pad_def
+  grounder.op_ids_def
+  grounder.op_prefix_pad_def
+  grounder.grounded_pred.simps
+  grounder.map_fact.simps
+  grounder.ga_pre.simps
+  grounder.ga_eff.simps
+  grounder.grounded_ac.simps
+  grounder.ground_dom_def
+  grounder.ground_prob_def
+  grounder.ground_ac_name.simps
+  grounder.fact_map_def
+declare pddl_ground_code[code]
 
 
 end
